theories/Dot/stamping/astStamping.v
@@ -2,7 +2,8 @@
     way, without involving Iris. *)
 From stdpp Require Import gmap.
 From D Require Import tactics.
-From D.Dot Require Import syn synLemmas typeExtractionSyn stampingDefsCore skeleton unstampedness_binding.
+From D.Dot Require Import syn synLemmas typeExtractionSyn stampingDefsCore
+  skeleton unstampedness_binding lr_syn_aux.
 
 Set Implicit Arguments.
 
