theories/Dot/syn/lr_syn_aux.v
@@ -1,0 +1,307 @@
+(**
+Syntactic predicates used to define our logical relation for DOT,
+and misc. useful lemmas.
+*)
+From D Require Export prelude.
+From iris.program_logic Require Import language.
+From D.Dot Require Export syn rules.
+
+Implicit Types
+         (L T U: ty) (v: vl) (e: tm) (d: dm) (ds: dms) (p : path)
+         (Γ : ctx) (ρ : env) (Pv : vl → Prop).
+
+Unset Program Cases.
+
+Lemma tskip_subst i e s: (iterate tskip i e).|[s] = iterate tskip i e.|[s].
+Proof. exact: cons_subst. Qed.
+
+Lemma TLater_subst i T s: (iterate TLater i T).|[s] = iterate TLater i T.|[s].
+Proof. exact: cons_subst. Qed.
+
+Lemma path2tm_subst p ρ: (path2tm p).|[ρ] = path2tm p.|[ρ].
+Proof. by elim: p => /= [//|p -> l]. Qed.
+
+(******************************************************************************)
+(** [path_wp], but for Coq predicates. *)
+(******************************************************************************)
+
+Inductive path_wp_pure : path → (vl → Prop) → Prop :=
+| pwp_pv vp Pv : Pv vp → path_wp_pure (pv vp) Pv
+| pwp_pself p vp q l Pv : path_wp_pure p (eq vp) → vp @ l ↘ dpt q → path_wp_pure q Pv →
+  path_wp_pure (pself p l) Pv .
+Local Hint Constructors path_wp_pure : core.
+
+Lemma path_wp_pure_inv_pv Pv v : path_wp_pure (pv v) Pv ↔ Pv v.
+Proof. split; by [inversion_clear 1 | auto]. Qed.
+
+Lemma path_wp_pure_inv_pself Pv p l : path_wp_pure (pself p l) Pv →
+  ∃ vp q, path_wp_pure p (eq vp) ∧ vp @ l ↘ dpt q ∧ path_wp_pure q Pv ∧
+  path_wp_pure (pself p l) Pv.
+Proof. inversion_clear 1; naive_solver. Qed.
+
+Global Instance Proper_pwp_pure: Proper ((=) ==> pointwise_relation _ iff ==> iff) path_wp_pure.
+Proof.
+  (* The induction works best in this shape, but this instance is best kept local. *)
+  have Proper_pwp_2: ∀ p, Proper (pointwise_relation _ iff ==> iff) (path_wp_pure p).
+  by rewrite /pointwise_relation => p P1 P2 HPeq; split;
+    induction 1; naive_solver.
+  solve_proper.
+Qed.
+
+Lemma path_wp_pure_wand {Pv1 Pv2 p}:
+  path_wp_pure p Pv1 →
+  (∀ v, Pv1 v → Pv2 v) →
+  path_wp_pure p Pv2.
+Proof. elim; eauto. Qed.
+
+Lemma path_wp_pure_eq p Pv :
+  path_wp_pure p Pv ↔ ∃ v, path_wp_pure p (eq v) ∧ Pv v.
+Proof.
+  split.
+  - elim; naive_solver.
+  - move => [v [Hpeq HPv]]. dependent induction Hpeq; naive_solver.
+Qed.
+
+Lemma path_wp_pure_det {p v1 v2}:
+  path_wp_pure p (eq v1) →
+  path_wp_pure p (eq v2) →
+  v1 = v2.
+Proof.
+  move => Hp1 Hp2; move: v2 Hp2; induction Hp1; intros; inverse Hp2; first naive_solver.
+  lazymatch goal with H1 : ?vp @ l ↘ dpt ?q, H2 : ?vp0 @ l ↘ dpt ?q0 |- _ =>
+    (suff ?: q = q0 by subst; auto);
+    (suff ?: vp = vp0 by subst; objLookupDet);
+    auto
+  end.
+Qed.
+
+Lemma path_wp_pure_swap p w :
+  path_wp_pure p (λ v, v = w) ↔
+  path_wp_pure p (eq w).
+Proof. split => Hp; exact: path_wp_pure_wand. Qed.
+
+Lemma path_wp_exec_pure p v :
+  path_wp_pure p (eq v) →
+  ∃ n, PureExec True n (path2tm p) (tv v).
+Proof.
+  move HE: (eq v) => P Hp; move: v HE; induction Hp; intros; simplify_eq.
+  by exists 0; constructor.
+  have [m /(_ I) Hs1] := IHHp1 _ eq_refl.
+  have [n /(_ I) Hs2] := IHHp2 _ eq_refl.
+  exists (S m + n) => _ /=.
+  eapply (nsteps_trans (S m)), Hs2; eapply nsteps_r.
+  by apply (pure_step_nsteps_ctx (fill_item (ProjCtx l))), Hs1.
+  by apply nsteps_once_inv, pure_tproj.
+Qed.
+
+Lemma PureExec_to_terminates n φ e v : PureExec φ n e (tv v) → φ → terminates e.
+Proof. intros HP Hφ. exists v. eapply nsteps_rtc, HP, Hφ. Qed.
+
+Definition alias_paths p q :=
+  path_wp_pure q (λ vp, path_wp_pure p (eq vp)).
+
+Lemma alias_paths_pv_eq_1 p vr :
+  alias_paths p (pv vr) ↔ path_wp_pure p (eq vr).
+Proof. rewrite /alias_paths. by setoid_rewrite path_wp_pure_inv_pv. Qed.
+
+Hint Extern 1 (path_wp_pure _ _) => by apply path_wp_pure_swap : core.
+
+Lemma alias_paths_pv_eq_2 p vr :
+  alias_paths (pv vr) p ↔ path_wp_pure p (eq vr).
+Proof.
+  rewrite /alias_paths -path_wp_pure_swap.
+  by setoid_rewrite path_wp_pure_inv_pv.
+Qed.
+
+Lemma alias_paths_self p v :
+  alias_paths p (pv v) → alias_paths p p.
+Proof.
+  rewrite alias_paths_pv_eq_1 /alias_paths !path_wp_pure_eq; naive_solver.
+Qed.
+
+Lemma alias_paths_refl_vl v :
+  alias_paths (pv v) (pv v).
+Proof. hnf; eauto. Qed.
+
+Lemma alias_paths_sameres p q:
+  alias_paths p q ↔
+  ∃ v,
+    path_wp_pure p (eq v) ∧
+    path_wp_pure q (eq v).
+Proof. rewrite /alias_paths !path_wp_pure_eq; naive_solver. Qed.
+
+Lemma alias_paths_symm p q :
+  alias_paths p q ↔ alias_paths q p.
+Proof. rewrite !alias_paths_sameres. naive_solver. Qed.
+Lemma alias_paths_symm' p q :
+  alias_paths p q → alias_paths q p.
+Proof. apply alias_paths_symm. Qed.
+
+Lemma alias_paths_trans p q r :
+  alias_paths p q → alias_paths q r → alias_paths p r.
+Proof.
+  rewrite !alias_paths_sameres => -[v [Hpv Hqv]] [w [Hqw Hrw]].
+  have Heq: v = w by exact: path_wp_pure_det. simplify_eq; eauto.
+Qed.
+
+Lemma alias_paths_samepwp_pure p q:
+  alias_paths p q ↔
+    (∃ u, path_wp_pure p (eq u)) ∧
+    ∀ Pv, path_wp_pure p Pv ↔ path_wp_pure q Pv.
+Proof.
+  rewrite alias_paths_sameres; split.
+  - destruct 1 as (v & Hp & Hq).
+    split. by eauto. intros Pv.
+    rewrite !path_wp_pure_eq.
+    f_equiv => w; split => -[Hr];
+      [ rewrite -(path_wp_pure_det Hp Hr)
+      | rewrite -(path_wp_pure_det Hq Hr)]; auto.
+  - intros [[u Hp] Heq]. exists u.
+    split; by [|rewrite -Heq].
+Qed.
+
+Lemma alias_paths_elim_eq_pure Pv {p q}:
+  alias_paths p q →
+  path_wp_pure p Pv ↔ path_wp_pure q Pv.
+Proof. move => /alias_paths_samepwp_pure [_]. apply. Qed.
+
+(******************************************************************************)
+(** For primitives. *)
+(******************************************************************************)
+Definition prim_sem (B : base_ty) :=
+  match B with
+  | tbool => bool
+  | tnat => nat
+  end.
+
+Definition prim_evals_to (B : base_ty) (v : vl) : prim_sem B → Prop :=
+  match B return prim_sem B → Prop with
+  | tbool => λ l, v = vlit $ lbool l
+  | tnat  => λ l, v = vlit $ lnat l
+  end.
+
+Definition pure_interp_prim B v := ∃ l : prim_sem B, prim_evals_to B v l.
+
+(******************************************************************************)
+(** For definition typing. *)
+(******************************************************************************)
+
+Definition label_of_ty T : option label :=
+  match T with
+  | TTMem l _ _ => Some l
+  | TVMem l _ => Some l
+  | _ => None
+  end.
+
+(** Context extension for use with definition typing, as in
+    [Γ |L V ⊨d d : T] and [Γ |L V ⊨ds ds : T]. *)
+Definition defCtxCons Γ V := TLater V :: Γ.
+Notation "Γ |L V" := (defCtxCons Γ V) (at level 60).
+
+Lemma norm_selfSubst ds s: selfSubst ds.|[up s] = ds.|[(vobj ds).[s] .: s].
+Proof. by rewrite /selfSubst up_sub_compose. Qed.
+
+(** Presence and absence of definitions. *)
+Definition dms_has ds l d := dms_lookup l ds = Some d.
+Definition dms_hasnt ds l := dms_lookup l ds = None.
+
+Lemma dms_hasnt_map ds l f:
+  dms_hasnt ds l →
+  dms_hasnt (map (mapsnd f) ds) l.
+Proof.
+  elim: ds => //; rewrite /dms_hasnt/mapsnd/= => [[l' d] ds IHds H].
+  by case_decide; eauto 2.
+Qed.
+
+Lemma dms_hasnt_subst l ds ρ : dms_hasnt ds l → dms_hasnt ds.|[ρ] l.
+Proof. apply dms_hasnt_map. Qed.
+
+Lemma dms_lookup_head l d ds: dms_lookup l ((l, d) :: ds) = Some d.
+Proof. by cbn; case_decide. Qed.
+
+Lemma dms_lookup_mono l l' d d' ds:
+  dms_hasnt ds l →
+  dms_lookup l' ds = Some d' →
+  dms_lookup l' ((l, d) :: ds) = Some d'.
+Proof.
+  rewrite /dms_hasnt /= => Hlds Hl; by case_decide; simplify_eq.
+Qed.
+
+Lemma dms_hasnt_notin_eq l ds : dms_hasnt ds l ↔ l ∉ map fst ds.
+Proof.
+  elim: ds => [|[l' d] ds] /=; first by split; [inversion 2|].
+  rewrite /dms_hasnt/= not_elem_of_cons => IHds. case_decide; naive_solver.
+Qed.
+
+(** Well-formedness of definition lists. *)
+Notation wf_ds ds := (NoDup (map fst ds)).
+
+(** Definitions [ds] appear in the object resulting from evaluating path [ p.|[ρ] ]. *)
+Definition path_includes p ρ ds :=
+  path_wp_pure p.|[ρ] (λ w, ∃ ds', w = vobj ds' ∧ ds.|[ρ] `sublist_of` ds'.|[w/] ∧ wf_ds ds').
+
+Lemma ds_notin_subst l ds ρ :
+  l ∉ map fst ds →
+  l ∉ map fst ds.|[ρ].
+Proof.
+  (* elim: ds => [//|[l' d] ds IH]; cbn.
+  rewrite !not_elem_of_cons. naive_solver. *)
+  intros; by apply dms_hasnt_notin_eq, dms_hasnt_subst, dms_hasnt_notin_eq.
+Qed.
+
+Lemma wf_ds_nil : wf_ds ([] : dms). Proof. constructor. Qed.
+Hint Resolve wf_ds_nil : core.
+
+Lemma wf_ds_sub ds ρ : wf_ds ds → wf_ds ds.|[ρ].
+Proof.
+  elim: ds => [//=|[l d] ds IH]; cbn.
+  inversion_clear 1; constructor; last by eauto.
+  exact: ds_notin_subst.
+Qed.
+
+Lemma path_includes_self ds ρ : wf_ds ds → path_includes (pv (ids 0)) (vobj ds.|[up ρ] .: ρ) ds.
+Proof.
+  by constructor; exists ds.|[up ρ]; rewrite /= up_sub_compose; split_and!;
+    last apply wf_ds_sub.
+Qed.
+
+Lemma path_includes_split p ρ l d ds :
+  path_includes p ρ ((l, d) :: ds) →
+  path_includes p ρ [(l, d)] ∧
+  path_includes p ρ ds.
+Proof.
+  rewrite /path_includes !path_wp_pure_eq; cbn.
+  intros (v & Hpw & ds' & -> & ((k1 & k2 & Hpid & Hpids)%sublist_cons_l & Hno)).
+  repeat (split_and! => //; try eexists); rewrite Hpid; apply sublist_inserts_l.
+  by apply sublist_skip, sublist_nil_l.
+  by apply sublist_cons, Hpids.
+Qed.
+
+Lemma dms_has_in_eq l d ds : wf_ds ds →
+  dms_has ds l d ↔ (l, d) ∈ ds.
+Proof.
+  rewrite /dms_has; elim: ds => [Hwf|[l' d'] ds IH /= /NoDup_cons [Hni Hwf]];
+    [by split; [|inversion 1]| rewrite elem_of_cons].
+  case_decide; first split; first 1 last; [|naive_solver..].
+  destruct 1; simplify_eq/=; [naive_solver|destruct Hni].
+  by eapply elem_of_list_In, (in_map fst ds (_,_)), elem_of_list_In.
+Qed.
+
+Lemma dms_lookup_sublist l p ds :
+  wf_ds ds → [(l, dpt p)] `sublist_of` ds →
+  dms_lookup l ds = Some (dpt p).
+Proof.
+  rewrite sublist_cons_l; intros Hwf ?; ev; simplify_eq/=.
+  apply dms_has_in_eq; [done|].
+  rewrite elem_of_app elem_of_cons. naive_solver.
+Qed.
+
+Lemma path_includes_field_aliases p ρ l v :
+  path_includes p ρ [(l, dpt (pv v))] →
+  alias_paths (pself p.|[ρ] l) (pv v.[ρ]).
+Proof.
+  rewrite /path_includes/alias_paths/= !path_wp_pure_eq;
+    intros (w & Hwp & ds & -> & Hsub & Hwf').
+  enough (dms_lookup l (selfSubst ds) = Some (dpt (pv v.[ρ]))) by eauto 10.
+  apply dms_lookup_sublist, Hsub. exact: wf_ds_sub.
+Qed.
